src/FlatModel.v
@@ -54,7 +54,7 @@ Definition code_writes (c : list ast) :=
   let '(ws, _) :=
       fold_left (fun '(ws, next_loc) a =>
                    ((0, 0,
-                     {| write_id := 0;
+                     {| write_id := MemWriteID 0;
                         write_footprint := {| Types.location := next_loc; Types.size := 4 |};
                         write_val := unsafe_encode a ;
                         write_kind := WKNormal |})::ws,
@@ -66,45 +66,17 @@ Definition code_writes (c : list ast) :=
 (* Head of the [list nat] is MSB *)
 Definition data_writes (ds : list (nat * list nat)) :=
   List.map (fun '(loc, bytes) =>
-              (0, 0, {| write_id := 0;
+              (0, 0, {| write_id := MemWriteID 0;
                         write_footprint := {| Types.location := MemLoc loc;
                                               Types.size := List.length bytes |};
                         write_val := List.rev bytes;
                         write_kind := WKNormal |}))
            ds.
 
-Section NondetCallbacks.
-  Definition first_not_disabled : Model.nondet_callback :=
-    fun n c =>
-      match fold_left (fun 'res i =>
-                         match res, Fin.of_nat i n with
-                         | None, inleft i =>
-                           match c i with
-                           | Model.ERDisabled => None
-                           | res => Some res
-                           end
-                         | _, _ => res
-                         end)
-                      (List.seq 0 n)
-                      None with
-      | Some res => res
-      | None => Model.ERDisabled
-      end.
-End NondetCallbacks.
-
 Definition init_test
-           (mem : list (instruction_id_t * mem_write_id_t * mem_write))
+           (mem : list (thread_id * instruction_id * mem_write))
   :=
   Model.run mem [MemLoc 4096].
-
-Definition run_test
-           (ncall : Model.nondet_callback)
-           (dcall : Model.debug_callback)
-           (mem : list (instruction_id_t * mem_write_id_t * mem_write))
-           (bound : nat)
-  : Model.exec_result :=
-  Model.exec ncall dcall bound mem [MemLoc 4096].
-
 
 Existing Instance Model.showable_state.
 
@@ -147,8 +119,7 @@ Cd "extracted_ocaml".
 
 Separate Extraction
          ExtrOcamlIntConv.nat_of_int ExtrOcamlIntConv.int_of_nat
-         run_test show_state first_not_disabled
-         init_test Model.step
+         init_test Model.step show_state
          test_and test_str test_ldr.
 
 Cd "..".
